Undirected_Graphs/Berge.thy
@@ -3,7 +3,7 @@
 *)
 
 theory Berge
-imports Main "HOL-Library.Extended_Nat" "HOL-Eisbach.Eisbach_Tools"
+imports Main "../Misc/enat_misc" "HOL-Eisbach.Eisbach_Tools"
 begin
 
 subsection\<open>Paths, connected components, and symmetric differences\<close>
@@ -1153,18 +1153,6 @@ lemma card'_finite_nat[iff]: "(card' A = numeral m) \<longleftrightarrow> (finit
   by (simp add: numeral_eq_enat)
 
 (*TODO: remove the enat notions*)
-
-declare one_enat_def
-
-declare zero_enat_def
-
-lemma eval_enat_numeral:
-  "numeral Num.One = eSuc 0"
-  "numeral (Num.Bit0 n) = eSuc (numeral (Num.BitM n))"
-  "numeral (Num.Bit1 n) = eSuc (numeral (Num.Bit0 n))"
-  by (simp_all add: BitM_plus_one eSuc_enat numeral_plus_one[symmetric] zero_enat_def one_enat_def)
-
-declare eSuc_enat[symmetric, simp]
 
 lemma card'_finite_enat[iff]: "(card' A = enat m) \<longleftrightarrow> (finite A \<and> card A = m)"
   unfolding card'_def by simp
